Playing around with binary search trees

teaching/taltech2018/sol/BinarySearchTree.fst
@@ -8,7 +8,7 @@ private type btree =
 
 (* Search function / containment predicate for binary (search) trees *)
 
-private let rec btree_contains (t:btree) (n:nat) : bool =
+private let rec btree_contains (t:btree) (n:nat) : GTot bool =
   match t with 
   | Leaf -> false
   | Node t1 m t2 -> 
@@ -18,11 +18,11 @@ private let rec btree_contains (t:btree) (n:nat) : bool =
 
 (* Empty binary tree *)
 
-private let empty_btree () : btree = Leaf
+private let empty_btree () : GTot btree = Leaf
 
 (* Insertion into a binary (search) tree *)
 
-private let rec btree_insert (t:btree) (n:nat) : btree =
+private let rec btree_insert (t:btree) (n:nat) : GTot btree =
   match t with 
   | Leaf -> Node Leaf n Leaf
   | Node t1 m t2 -> 
@@ -32,21 +32,21 @@ private let rec btree_insert (t:btree) (n:nat) : btree =
 
 (* Sortedness predicate for binary (search) trees *)
 
-private let rec sorted_left_of (t:btree) (n:nat) : bool = 
+private let rec sorted_left_of (t:btree) (n:nat) : GTot bool = 
   match t with
   | Leaf -> true
   | Node t1 m t2 -> t1 `sorted_left_of` m && 
                     m < n && 
                     t2 `sorted_right_of` m
 
-and sorted_right_of (t:btree) (n:nat) : bool = 
+and sorted_right_of (t:btree) (n:nat) : GTot bool = 
   match t with
   | Leaf -> true
   | Node t1 m t2 -> t1 `sorted_left_of` m && 
                     m > n && 
                     t2 `sorted_right_of` m
 
-private let rec sorted (t:btree) : bool =
+private let rec sorted (t:btree) : GTot bool =
   match t with
   | Leaf -> true
   | Node t1 n t2 -> t1 `sorted_left_of` n && 
@@ -54,8 +54,9 @@ private let rec sorted (t:btree) : bool =
 
 (* Useful lemmas about sortedness and the tree operations defined above *)
 
-private let rec lemma_btree_insert_is_sorted (t:btree) (n:nat) : Lemma (requires (sorted t))
-                                                                       (ensures  (sorted (btree_insert t n))) = 
+private let rec lemma_btree_insert_is_sorted (t:btree) (n:nat) 
+  : Lemma (requires (sorted t))
+          (ensures  (sorted (btree_insert t n))) = 
   match t with
   | Leaf -> ()
   | Node t1 m t2 -> 
@@ -63,8 +64,9 @@ private let rec lemma_btree_insert_is_sorted (t:btree) (n:nat) : Lemma (requires
       if n < m then lemma_btree_insert_is_sorted t1 n
                else lemma_btree_insert_is_sorted t2 n
 
-private let rec lemma_btree_insert_exists (t:btree) (n:nat) : Lemma (requires (sorted t))
-                                                                    (ensures  ((btree_insert t n) `btree_contains` n)) =
+private let rec lemma_btree_insert_exists (t:btree) (n:nat) 
+  : Lemma (requires (sorted t))
+          (ensures  ((btree_insert t n) `btree_contains` n)) =
   match t with
   | Leaf -> ()
   | Node t1 m t2 -> 
@@ -72,8 +74,9 @@ private let rec lemma_btree_insert_exists (t:btree) (n:nat) : Lemma (requires (s
       if n < m then lemma_btree_insert_exists t1 n
                else lemma_btree_insert_exists t2 n
 
-private let rec lemma_exists_btree_insert_equal (t:btree) (n:nat) : Lemma (requires (sorted t && t `btree_contains` n))
-                                                                          (ensures  (btree_insert t n = t)) = 
+private let rec lemma_exists_btree_insert_equal (t:btree) (n:nat) 
+  : Lemma (requires (sorted t && t `btree_contains` n))
+          (ensures  (btree_insert t n = t)) = 
   match t with
   | Node t1 m t2 -> 
       if n = m then () else 
@@ -87,37 +90,43 @@ abstract type stree =
 
 (* Binary search tree operations, derived from tree operations defined above*)
 
-let contains (t:stree) (n:nat) : bool =
+let contains (t:stree) (n:nat) : GTot bool =
   btree_contains t n
 
-let empty () : stree = 
+let empty () : GTot stree = 
   empty_btree ()
 
-let insert (t:stree) (n:nat) : stree = 
+let insert (t:stree) (n:nat) : GTot stree = 
   lemma_btree_insert_is_sorted t n; 
   btree_insert t n
 
 (* Sanity check lemmas *)
 
-private let lemma_contains_equals (t:stree) (n:nat) : Lemma (t `btree_contains` n = t `contains` n) = 
+private let lemma_contains_equals (t:stree) (n:nat) 
+  : Lemma (t `btree_contains` n = t `contains` n) = 
   ()
 
-private let lemma empty_equals () : Lemma (empty_btree () = empty ()) = 
+private let lemma empty_equals () 
+  : Lemma (empty_btree () = empty ()) = 
   ()
 
-private let lemma_insert_equals (t:stree) (n:nat) : Lemma (btree_insert t n = insert t n) = 
+private let lemma_insert_equals (t:stree) (n:nat) 
+  : Lemma (btree_insert t n = insert t n) = 
   ()
   
 (* Important properties of binary search trees *)
 
-let rec lemma_insert_is_sorted (t:stree) (n:nat) : Lemma (sorted (btree_insert t n)) = 
+let rec lemma_insert_is_sorted (t:stree) (n:nat) 
+  : Lemma (sorted (btree_insert t n)) = 
   lemma_btree_insert_is_sorted t n
 
-let rec lemma_insert_exists (t:stree) (n:nat) : Lemma ((btree_insert t n) `btree_contains` n) =
+let rec lemma_insert_exists (t:stree) (n:nat) 
+  : Lemma ((btree_insert t n) `btree_contains` n) =
   lemma_btree_insert_exists t n
 
-let rec lemma_exists_insert_equal (t:stree) (n:nat) : Lemma (requires (t `btree_contains` n))
-                                                            (ensures  (btree_insert t n = t)) = 
+let rec lemma_exists_insert_equal (t:stree) (n:nat) 
+  : Lemma (requires (t `btree_contains` n))
+          (ensures  (btree_insert t n = t)) = 
   lemma_exists_btree_insert_equal t n
 
 
@@ -140,22 +149,23 @@ let heap = FStar.Heap.heap
 let sel h (r:treeptr) = FStar.Heap.sel h r
 let upd h (r:treeptr) v = FStar.Heap.upd h r v 
 
+let is_leaf (r:treeptr) (h:heap) = None? (sel h r)
+let is_node (r:treeptr) (h:heap) = Some? (sel h r)
+
 let rec is_stree (r:treeptr) (t:stree) (h:heap) : GTot bool (decreases t) =
   match t with 
-  | Leaf -> None? (sel h r)
+  | Leaf -> is_leaf r h
   | Node t1 n t2 -> 
-      Some? (sel h r) &&
+      is_node r h &&
       (match (sel h r) with
        | Some nd -> is_stree nd.left t1 h &&
                     n = nd.value &&
                     is_stree nd.right t2 h)
 
-let rec search (#t:erased stree) (r:treeptr) (n:nat) : ST bool (requires (fun h0 -> is_stree r (reveal t) h0))
-                                                        (ensures  (fun h0 b h1 -> 
-                                                                     h0 == h1 /\ 
-                                                                     (reveal t) `contains` n <==> b = true)) =
-  let nd = !r in 
-  match nd with 
+let rec search (#t:erased stree) (r:treeptr) (n:nat) 
+  : ST bool (requires (fun h0 -> is_stree r (reveal t) h0))
+            (ensures  (fun h0 b h1 -> h0 == h1 /\ (reveal t) `contains` n <==> b = true)) =
+  match !r with 
   | None -> false
   | Some nd -> 
       if n = nd.value then true else 
@@ -163,3 +173,12 @@ let rec search (#t:erased stree) (r:treeptr) (n:nat) : ST bool (requires (fun h0
                             search #t1 nd.left n)
                       else (let t2 = hide (match (reveal t) with | Node _ _ t2 -> t2) in
                             search #t2 nd.right n)
+
+let create () : ST treeptr (requires (fun _ -> True))
+                           (ensures  (fun _ r h1 -> is_leaf r h1)) =
+  alloc None
+
+let rec insert (#t:erased stree) (r:treeptr) (n:nat) 
+  : ST unit (requires (fun h0 -> is_stree r (reveal t) h0))
+            (ensures  (fun h0 _ h1 -> True))
+
